Checkpoint; typeclass search results in `bool_decide (k ∈ m)` being
definitionally false when `m` is a gmap. This was used this in defining
Go semantics, which resulted in (fortunately easy-to-notice) wrong
behavior.

new/golang/theory/pkg.v
@@ -1,3 +1,4 @@
+From New.golang.defn Require Import pkg.
 From New.golang.theory Require Import exception mem assume.
 From Perennial Require Import base.
 Import Ltac2. Import Printf.
@@ -8,28 +9,8 @@ Set Default Proof Using "Type".
 Section init_defns.
 Context `{ffi_sem: ffi_semantics} `{!ffi_interp ffi} `{!heapGS Σ} {go_ctx : GoContext}.
 
-Local Definition is_init_inv get_is_pkg_init : iProp Σ :=
-  inv nroot (
-      ∃ package_started package_inited,
-        "Hg" ∷ own_go_state package_inited ∗
-        (* NOTE: could own an auth that has precisely the "started" keys, and
-           the exclusive pointstos can be given to program proofs to help escrow
-           resources into initialization. *)
-        "#Hinit" ∷ □([∗ set] pkg_name ∈ package_inited, get_is_pkg_init pkg_name) ∗
-        "%Hpackage_inited" ∷ (⌜ ∀ pkg_name, g ("P" ++ pkg_name)%go =
-                                # <$> ((gset_to_gmap "initialized"%go package_inited) ∪
-                                   (gset_to_gmap "started"%go package_started)) !! pkg_name
-                                  ⌝)
-    ).
-
-(** [is_go_context] asserts that the implicit [GoContext] matches the execution
-    state of the current Go program. *)
-Definition is_go_context : iProp Σ :=
-  ∃ get_is_pkg_init, is_init_inv get_is_pkg_init.
-#[global] Opaque is_go_context.
-#[local] Transparent is_go_context.
-#[global] Instance : Persistent is_go_context.
-Proof. apply _. Qed.
+Definition is_init (σ : state) : Prop :=
+  σ.(go_state).(package_state) = ∅.
 
 (** [own_initializing] denotes permission to run [package.init]. This is
     exclusive because go packages are initialized sequentially, in a single
@@ -38,84 +19,28 @@ Proof. apply _. Qed.
     appropriate user-defined predicates is facilitated by [GetIsPkgInitWf]
     below. *)
 Definition own_initializing (get_is_pkg_init : go_string → iProp Σ) : iProp Σ :=
-  ∃ g, "#Hinv" ∷ is_init_inv get_is_pkg_init ∗ "Hg" ∷ own_globals (DfracOwn (1/2)) g.
+  ∃ package_inited,
+    "Hg" ∷ own_go_state package_inited ∗
+    (* NOTE: could own an auth that has precisely the "started" keys, and
+           the exclusive pointstos can be given to program proofs to help escrow
+           resources into initialization. *)
+    "#Hinit" ∷ □([∗ map] pkg_name ↦ (inited : bool) ∈ package_inited,
+                   if inited then get_is_pkg_init pkg_name else True).
 #[global] Opaque own_initializing.
 #[local] Transparent own_initializing.
 
 Lemma go_init get_is_pkg_init σ :
   is_init σ →
-  own_globals (DfracOwn 1) σ.(globals) ={⊤}=∗
-  own_initializing get_is_pkg_init ∗ is_go_context.
+  own_go_state σ.(go_state).(package_state) ={⊤}=∗
+  own_initializing get_is_pkg_init.
 Proof.
-  intros (Hvard & Hfuncs & Hmethod & Hpkg).
-  iIntros "[Hg Hg2]".
-  iFrame. iMod (inv_alloc with "[-]") as "#H".
-  2:{ by iFrame "H". }
-  iExists _, ∅, ∅. iFrame. rewrite big_sepS_empty. iFrame "#%".
-  done.
+  intros ->. iIntros "$". iModIntro. iModIntro. by iApply big_sepM_empty.
 Qed.
 
 End init_defns.
 
 Section package_init_and_defined.
 Context `{ffi_sem: ffi_semantics} `{!ffi_interp ffi} `{!heapGS Σ} {go_ctx : GoContext}.
-
-(** XXX: there are a lof of design questions around [is_pkg_defined].
-    - construct using ltac2 or Goose?
-    - have an Iris version of [is_pkg_defined] or only a pure version?
-    - should WpFuncCall/MethodCall take a transitive version of
-      [is_pkg_defined], or just a single package's?
-    - if pure, should there be new automation for solving [is_pkg_defined_pure]?
-      Use typeclasses? Would be annoying to maintain automation for this given
-      that there's already Iris automation for [is_pkg_init].
-    - If not pure, should one unfold [is_pkg_defined] to get access to the
-    - Should the transitive [is_pkg_defined] be kept sealed? Use [Opaque], and
-      locally make it [Transparent] where needed in program proofs?
-    - and more.
-    Moreover, many of these questions do not make a big difference to the
-    resulting user experience.
-
-    So, this implementation makes design decisions arbitrarily around these
-    questions. For instance, rather than using ltac2 to generate predicates (as
-    is done for [is_pkg_init]), the predicate is generated in Goose.
- *)
-
-(** Used as a parameter of the below so that this pure predicate can be referred
-    without needing a [heapGS]. *)
-Class IsPkgDefinedPure (pkg_name : go_string) :=
-  {
-    is_pkg_defined_pure_def : ∀ {go_ctx : GoContext}, Prop;
-  }.
-
-(** [IsPkgDefined] connects package names to a predicate which asserts that all
-    functions/methods from the package and all of its dependencies are
-    available.
-
-    The pure predicate is used as an assumption in closed theorems. The Iris
-    predicate is used as a precondition in specs for [<PACKAGE NAME>.initialize']. *)
-Class IsPkgDefined (pkg_name : go_string) `{!IsPkgDefinedPure pkg_name} :=
-  {
-    is_pkg_defined_def : ∀ {go_ctx : GoContext}, iProp Σ;
-    is_pkg_defined_boot : ∀ {go_ctx : GoContext},
-      is_pkg_defined_pure_def → is_go_context -∗ is_pkg_defined_def
-  }.
-Notation is_pkg_defined_pure := is_pkg_defined_pure_def.
-#[global] Arguments is_pkg_defined_pure (pkg_name) {_} {go_ctx}.
-#[global] Opaque is_pkg_defined_pure.
-
-Notation is_pkg_defined := is_pkg_defined_def.
-#[global] Arguments is_pkg_defined (pkg_name) {_ _} {go_ctx}.
-#[global] Opaque is_pkg_defined.
-
-(** Internal to Goose. This says that the package's declarations are accessible
-    (including functions, methods, and variables). This does not cover any
-    dependencies.  This should only be referring to by definitions in
-    generatedproof; do not use this manually in proofs. *)
-Definition is_pkg_defined_single pkg_name `{!PkgInfo pkg_name} : iProp Σ :=
-  "#Hctx" ∷ is_go_context ∗
-  "%Hdefined" ∷ ⌜ is_pkg_defined_pure_single pkg_name ⌝.
-#[global] Opaque is_pkg_defined_single.
-#[local] Transparent is_pkg_defined_single.
 
 (** [IsPkgInit] connects pkg names (really the full package path) to their
     post-initialization predicate. There should only be one instance for each
@@ -172,11 +97,8 @@ Global Arguments get_is_pkg_init_prop (pkg_name) {_} {_} (get_is_pkg_init).
 End package_init_and_defined.
 
 #[global] Hint Mode IsPkgInit - + : typeclass_instances.
-#[global] Hint Mode IsPkgDefined - - - - - - + - : typeclass_instances.
 #[global] Hint Mode GetIsPkgInitWf + - : typeclass_instances.
 
-Notation is_pkg_defined_pure := is_pkg_defined_pure_def.
-Notation is_pkg_defined := is_pkg_defined_def.
 Notation get_is_pkg_init_prop := get_is_pkg_init_prop_def.
 
 Ltac2 fail m := Control.throw (Tactic_failure (Some m)).
@@ -190,7 +112,7 @@ Local Ltac2 build_pkg_init_deps name :=
          | cons ?pkg ?deps =>
              let rest := build_iprop deps in
              constr:((is_pkg_init $pkg ∗ $rest)%I)
-         | nil => constr:((is_pkg_defined $name ∗ is_go_context)%I)
+         | nil => constr:(True%I)
          | _ =>
              Message.print (Message.of_constr deps);
              fail (fprintf "build_pkg_init_deps: unable to match deps list")
@@ -242,145 +164,14 @@ Ltac2 build_get_is_pkg_init_wf () :=
 
 Notation "'build_get_is_pkg_init_wf'" := (ltac2:(build_get_is_pkg_init_wf ())) (only parsing).
 
-Section calls.
-Context `{ffi_sem: ffi_semantics} `{!ffi_interp ffi} `{!heapGS Σ} `{!GoContext}.
-
-Definition func_callv_def (func_name : go_string) : func.t :=
-  {|
-    func.f := <>;
-                func.x := "firstArg";
-    func.e := option.unwrap (GlobalGet (# "F"%go + # func_name)) "firstArg"
-  |}.
-Program Definition func_callv := sealed @func_callv_def.
-Definition func_callv_unseal : func_callv = _ := seal_eq _.
-
-
-Global Instance wp_func_callv (func_name : go_string) :
-  PureWp True (func_call #func_name)%E #(func_callv func_name)%E.
-Proof.
-  rewrite func_call_unseal /func_call_def func_callv_unseal.
-  intros ?????. iIntros "Hwp". wp_pure_lc "?".
-  wp_pures. by iApply "Hwp".
-Qed.
-
-Definition method_callv_def (type_id method_name : go_string) (receiver : val) : func.t :=
-  {|
-    func.f := <>;
-                func.x := "firstArg";
-    func.e :=
-      option.unwrap (GlobalGet (# "M"%go + # type_id + # "."%go + # method_name)) receiver "firstArg"
-  |}.
-Program Definition method_callv := sealed @method_callv_def.
-Definition method_callv_unseal : method_callv = _ := seal_eq _.
-
-Global Instance wp_method_callv (type_id method_name : go_string) (receiver : val) :
-  PureWp True (method_call #type_id #method_name receiver) #(method_callv type_id method_name receiver).
-Proof.
-  rewrite method_call_unseal /method_call_def method_callv_unseal.
-  intros ?????. iIntros "Hwp". wp_pure_lc "?".
-  wp_pures. by iApply "Hwp".
-Qed.
-
-(** Internal-ish to Goose. Users should never manually define instances of this.
-    The [P] predicate will generally be a package's [is_pkg_defined]. *)
-Class WpFuncCall func_name (f : val) (P : iProp Σ) :=
-  wp_func_call :
-    (∀ (first_arg : val) Φ,
-       P -∗ (WP (f first_arg) {{ Φ }}) -∗
-       WP #(func_callv func_name) first_arg {{ Φ }}).
-
-(** Same as [WpFuncCall]. *)
-Class WpMethodCall (type_id : go_string) (func_name : go_string) (m : val) (P : iProp Σ)
-  := wp_method_call :
-    (∀ (first_arg receiver : val) Φ,
-         P -∗ (WP (m receiver first_arg) {{ Φ }}) -∗
-         WP #(method_callv type_id func_name receiver) first_arg {{ Φ }}).
-
-#[local] Transparent is_go_context.
-
-Lemma wp_globals_get var_name :
-  {{{ is_go_context }}} (globals.get #var_name) {{{ RET #(global_addr var_name); True }}}.
-Proof.
-  iIntros (?) "#Hctx HΦ". rewrite globals.get_unseal.
-  iNamed "Hctx". wp_call_lc "Hlc". wp_bind. iNamed "Hctx".
-  iInv "Hctx" as "Hi" "Hclose".
-  iMod (lc_fupd_elim_later with "[$] Hi") as "Hi". iNamed "Hi".
-  rewrite [in #(_ :: var_name)]to_val_unseal.
-  wp_apply (wp_GlobalGet with "[$]").
-  iIntros "Hg".
-  iMod ("Hclose" with "[Hg Hinit]").
-  { iFrame "∗#%". }
-  iModIntro.
-  rewrite Hglobal_addr.
-  wp_pures. by iApply "HΦ".
-Qed.
-
-#[local] Transparent is_pkg_defined_single.
-
-(** Internal to Goose. Used in generatedproofs to establish [WpFuncCall]. *)
-Lemma wp_func_call' {func_name func} `{!PkgInfo pkg_name} P :
-  (is_pkg_defined_pure_single pkg_name → __function func_name = Some func) →
-  (P -∗ is_pkg_defined_single pkg_name) →
-  WpFuncCall func_name func P.
-Proof.
-  intros Hlookup HP. rewrite /WpFuncCall. iIntros "* Hdef HΦ". rewrite func_callv_unseal.
-  wp_pure_lc "Hlc". wp_pures. wp_bind. iDestruct (HP with "Hdef") as "Hdef". iNamed "Hdef". iNamed "Hctx".
-  iInv "Hctx" as "Hi" "Hclose". iMod (lc_fupd_elim_later with "[$] Hi") as "Hi".
-  iNamed "Hi". rewrite [in #(_ :: _)]to_val_unseal. wp_apply (wp_GlobalGet with "[$]").
-  iIntros "Hg". iMod ("Hclose" with "[Hg Hinit]"). { iFrame "∗#%". }
-  iModIntro. rewrite Hfunction.
-  rewrite Hlookup //. wp_pures. iApply "HΦ".
-Qed.
-
-(** Internal to Goose. Used in generatedproofs to establish [WpMethodCall]. *)
-Lemma wp_method_call' {type_id method_name m} `{!PkgInfo pkg_name} P :
-  (is_pkg_defined_pure_single pkg_name → __method type_id method_name = Some m) →
-  (P -∗ is_pkg_defined_single pkg_name) →
-  WpMethodCall type_id method_name m P.
-Proof.
-  intros Hlookup HP. rewrite /WpMethodCall. iIntros "* Hdef HΦ". rewrite method_callv_unseal.
-  wp_pure_lc "Hlc". wp_pures. wp_bind. iDestruct (HP with "Hdef") as "Hdef". iNamed "Hdef".
-  iNamed "Hctx". iInv "Hctx" as "Hi" "Hclose". iMod (lc_fupd_elim_later with "[$] Hi") as "Hi".
-  iNamed "Hi". rewrite [in # (_ :: _)]to_val_unseal. wp_apply (wp_GlobalGet with "[$]").
-  iIntros "Hg". iMod ("Hclose" with "[Hg Hinit]"). { iFrame "∗#%". }
-  iModIntro. rewrite -app_assoc. rewrite Hmethod Hlookup //. wp_pures.
-  iApply "HΦ".
-Qed.
-
-End calls.
-
-Global Hint Mode WpMethodCall - - - - - - + + - - : typeclass_instances.
-Global Hint Mode WpFuncCall - - - - - - + - - : typeclass_instances.
-
-(* TODO: better error messages if tc_solve fails to find a val for the name. *)
-Tactic Notation "wp_globals_get_core" :=
-  wp_bind (globals.get _ _);
-  unshelve iApply (wp_globals_get with "[]").
-
-Tactic Notation "wp_func_call_core" :=
-  (wp_bind (#(func_callv _) _);
-   unshelve iApply (wp_func_call with "[]");
-   [| | (tc_solve || fail "could not find mapping from function name to val") | | ]).
-
-Tactic Notation "wp_method_call_core" :=
-  (wp_bind (#(method_callv _ _ _) _);
-   unshelve iApply (wp_method_call with "[]");
-   [| | (tc_solve || fail "could not find mapping from method to val") | |]).
-
 #[global]
 Notation "@! func" :=
-  #(func_callv func) (at level 1, no associativity, format "@! func") : expr_scope.
+  #(functions func []) (at level 1, no associativity, format "@! func") : expr_scope.
 
 #[global]
 Notation "rcvr @ type @ method" :=
-  #(method_callv type method #rcvr)
+  #(methods type method #rcvr)
     (at level 1, type at next level, no associativity) : expr_scope.
-
-Ltac solve_wp_func_call :=
-  apply wp_func_call'; [reflexivity| iIntros "H"; try iDestruct "H" as "[H _]"; iFrame "H"].
-
-Ltac solve_wp_method_call :=
-  apply wp_method_call'; [reflexivity | iIntros "H"; try iDestruct "H" as "[H _]"; iFrame "H"].
 
 (* FIXME: better implementation using PkgInfo to direct the search. Could try lithium even. *)
 (* solve a goal which is just [is_pkg_init] or [is_pkg_defined] *)
@@ -388,9 +179,7 @@ Ltac solve_pkg_init :=
   unfold named;
   lazymatch goal with
   | |- environments.envs_entails ?env (is_pkg_init _) => idtac
-  | |- environments.envs_entails ?env (is_pkg_defined _) => idtac
-  | |- environments.envs_entails ?env (is_go_context) => idtac
-  | _ => fail "not a is_pkg_init, is_pkg_defined, or is_go_context goal"
+  | _ => fail "not a is_pkg_init goal"
   end;
   try iAssumption;
   iClear "∗";
@@ -434,7 +223,8 @@ Lemma wp_package_init (pkg_name : go_string) `{!PkgInfo pkg_name} (init_func : v
   WP package.init pkg_name init_func #() {{ Φ }}.
 Proof.
   intros ? Heq. subst. iIntros "(Hown & Hpre) HΦ". rewrite package.init_unseal.
-  wp_call. wp_call_lc "Hlc".
+  wp_call.
+  wp_call_lc "Hlc".
   wp_bind. iNamed "Hown". iInv "Hinv" as "Hi" "Hclose".
   iMod (lc_fupd_elim_later with "[$] Hi") as "Hi". iRename "Hg" into "Hg2". iNamed "Hi".
   rewrite [in #(_ :: _)]to_val_unseal.
